src/FlatIntTagComp.v
@@ -1,0 +1,428 @@
+Require Import compcert.lib.Integers.
+Require Import ZArith.
+
+Require Import Common Monads.
+Require Import Metadata.
+Require String.
+Require FlatExprRet FlatIntTag.
+Require Import ListLemmas.
+Require HighValues HigherValue.
+
+Require Import Psatz.
+
+Module A := FlatExprRet.
+Module B := FlatIntTag.
+
+Module V1 := HigherValue.
+Module V2 := HighValues.
+
+Add Printing Constructor A.frame.
+Add Printing Constructor B.frame.
+
+
+Section compile.
+Open Scope option_monad.
+Open Scope Z_scope.
+
+Fixpoint numbered {A} base xs : list (Z * A) :=
+    match xs with
+    | [] => []
+    | x :: xs => (base, x) :: numbered (Z.succ base) xs
+    end.
+
+Definition nat_to_int n :=
+    let z := Z.of_nat n in
+    if Z_lt_dec z Int.modulus
+        then Some (Int.repr z)
+        else None.
+
+Definition compile_expr : A.expr -> B.expr :=
+    let fix go e :=
+        match e with
+        | A.Arg => B.Arg
+        | A.Self => B.Self
+        | A.Var i => B.Var i
+        | A.Deref e off => B.Deref (go e) off
+        end in go.
+
+Definition compile : A.stmt -> option B.stmt :=
+    let go_expr := compile_expr in
+    let fix go e :=
+        let fix go_list (es : list A.stmt) : option (list B.stmt) :=
+            match es with
+            | [] => Some []
+            | e :: es => @cons _ <$> go e <*> go_list es
+            end in
+        match e with
+        | A.Skip => Some B.Skip
+        | A.Seq s1 s2 => B.Seq <$> go s1 <*> (go s2)
+        | A.Call dst f a => Some (B.Call dst (go_expr f) (go_expr a))
+        | A.MkConstr dst tag args =>
+                nat_to_int tag >>= fun tag' =>
+                Some (B.MkConstr dst tag' (map go_expr args))
+        | A.Switch dst cases =>
+                go_list cases >>= fun cases' =>
+                Some (B.Switch dst (numbered 0 cases'))
+        | A.MkClose dst fname free =>
+                Some (B.MkClose dst fname (map go_expr free))
+        | A.Assign dst src => Some (B.Assign dst (go_expr src))
+        end in go.
+
+Definition compile_list :=
+    let go := compile in
+    let fix go_list es :=
+        match es with
+        | [] => Some []
+        | e :: es => @cons _ <$> go e <*> go_list es
+        end in go_list.
+
+End compile.
+
+Ltac refold_compile :=
+    fold compile_expr in *;
+    fold compile_list in *.
+
+
+
+Inductive I_expr : A.expr -> B.expr -> Prop :=
+| IArg : I_expr A.Arg B.Arg
+| ISelf : I_expr A.Self B.Self
+| IVar : forall i, I_expr (A.Var i) (B.Var i)
+| IDeref : forall ae be off,
+        I_expr ae be ->
+        I_expr (A.Deref ae off) (B.Deref be off)
+.
+
+Inductive I_stmt : A.stmt -> B.stmt -> Prop :=
+| ISkip :
+        I_stmt A.Skip B.Skip
+| ISeq : forall as1 as2 bs1 bs2,
+        I_stmt as1 bs1 ->
+        I_stmt as2 bs2 ->
+        I_stmt (A.Seq as1 as2) (B.Seq bs1 bs2)
+| ICall : forall dst af aa bf ba,
+        I_expr af bf ->
+        I_expr aa ba ->
+        I_stmt (A.Call dst af aa) (B.Call dst bf ba)
+| IMkConstr : forall dst atag aargs btag bargs,
+        Z.of_nat atag = Int.unsigned btag ->
+        Forall2 I_expr aargs bargs ->
+        I_stmt (A.MkConstr dst atag aargs) (B.MkConstr dst btag bargs)
+| ISwitch : forall dst acases bcases,
+        Forall2 I_stmt acases bcases ->
+        I_stmt (A.Switch dst acases) (B.Switch dst (numbered 0 bcases))
+| IMkClose : forall dst fname afree bfree,
+        Forall2 I_expr afree bfree ->
+        I_stmt (A.MkClose dst fname afree) (B.MkClose dst fname bfree)
+| IAssign : forall dst asrc bsrc,
+        I_expr asrc bsrc ->
+        I_stmt (A.Assign dst asrc) (B.Assign dst bsrc)
+.
+Hint Resolve ISkip.
+
+Inductive I_func : (A.stmt * A.expr) -> (B.stmt * B.expr) -> Prop :=
+| IFunc : forall acode aret bcode bret,
+        I_stmt acode bcode ->
+        I_expr aret bret ->
+        I_func (acode, aret) (bcode, bret).
+
+Inductive I_value : V1.value -> V2.value -> Prop :=
+| IConstr : forall atag aargs btag bargs,
+        Z.of_nat atag = Int.unsigned btag ->
+        Forall2 I_value aargs bargs ->
+        I_value (V1.Constr atag aargs) (V2.Constr btag bargs)
+| IClose : forall afname afree bfname bfree,
+        Pos.of_succ_nat afname = bfname ->
+        Forall2 I_value afree bfree ->
+        I_value (V1.Close afname afree) (V2.Close bfname bfree)
+.
+
+Inductive I_frame : A.frame -> B.frame -> Prop :=
+| IFrame : forall aarg aself alocals barg bself blocals,
+        I_value aarg barg ->
+        I_value aself bself ->
+        Forall2 (fun ap bp => fst ap = fst bp /\ I_value (snd ap) (snd bp)) alocals blocals ->
+        I_frame (A.Frame aarg aself alocals) (B.Frame barg bself blocals).
+Hint Constructors I_frame.
+
+Inductive I_cont : A.cont -> B.cont -> Prop :=
+| IkSeq : forall acode ak bcode bk,
+        I_stmt acode bcode ->
+        I_cont ak bk ->
+        I_cont (A.Kseq acode ak)
+               (B.Kseq bcode bk)
+| IkSwitch : forall ak bk,
+        I_cont ak bk ->
+        I_cont (A.Kswitch ak)
+               (B.Kswitch bk)
+| IkReturn : forall aret ak bret bk,
+        I_expr aret bret ->
+        I_cont ak bk ->
+        I_cont (A.Kreturn aret ak)
+               (B.Kreturn bret bk)
+| IkCall : forall dst af ak bf bk,
+        I_frame af bf ->
+        I_cont ak bk ->
+        I_cont (A.Kcall dst af ak)
+               (B.Kcall dst bf bk)
+| IkStop : forall aret bret,
+        I_expr aret bret ->
+        I_cont (A.Kstop aret)
+               (B.Kstop bret).
+
+Inductive I : A.state -> B.state -> Prop :=
+| IRun : forall acode af ak  bcode bf bk,
+        I_stmt acode bcode ->
+        I_frame af bf ->
+        I_cont ak bk ->
+        I (A.Run acode af ak)
+          (B.Run bcode bf bk)
+
+| IReturn : forall av ak bv bk,
+        I_value av bv ->
+        I_cont ak bk ->
+        I (A.Return av ak)
+          (B.Return bv bk)
+
+| IStop : forall av bv,
+        I_value av bv ->
+        I (A.Stop av) (B.Stop bv).
+
+
+
+Lemma compile_I_expr : forall a b,
+    compile_expr a = b ->
+    I_expr a b.
+induction a;
+intros0 Hcomp; simpl in Hcomp; try rewrite <- Hcomp; refold_compile;
+try solve [econstructor; eauto].
+Qed.
+
+Lemma map_compile_I_expr : forall a b,
+    map compile_expr a = b ->
+    Forall2 I_expr a b.
+induction a;
+intros0 Hcomp; simpl in Hcomp; try rewrite <- Hcomp; refold_compile;
+try solve [econstructor; eauto using compile_I_expr].
+Qed.
+
+Theorem compile_I_stmt : forall a b,
+    compile a = Some b ->
+    I_stmt a b.
+induction a using A.stmt_rect_mut with
+    (Pl := fun a => forall b,
+        compile_list a = Some b ->
+        Forall2 I_stmt a b);
+intros0 Hcomp; simpl in Hcomp; break_bind_option; inject_some; refold_compile;
+try solve [econstructor; eauto using compile_I_expr, map_compile_I_expr].
+
+- constructor.
+  + unfold nat_to_int in *. break_if; try discriminate.
+    inject_some.
+    rewrite Int.unsigned_repr; eauto.
+    unfold Int.max_unsigned. lia.
+  + eauto using map_compile_I_expr.
+Qed.
+
+
+
+Ltac i_ctor := intros; econstructor; simpl; eauto.
+Ltac i_lem H := intros; eapply H; simpl; eauto.
+
+Ltac stk_simpl := compute [
+    A.set  A.arg A.self A.locals
+    B.set  B.arg B.self B.locals
+    ] in *.
+
+Lemma set_I_frame : forall af bf dst av bv,
+    I_frame af bf ->
+    I_value av bv ->
+    I_frame (A.set af dst av) (B.set bf dst bv).
+intros0 II IIval. invc II.
+stk_simpl. constructor; eauto.
+Qed.
+Hint Resolve set_I_frame.
+
+Hint Constructors B.eval.
+
+Lemma local_sim : forall af bf l av,
+    I_frame af bf ->
+    A.local af l = Some av ->
+    exists bv,
+        B.local bf l = Some bv /\
+        I_value av bv.
+destruct af, bf.
+make_first locals. induction locals; intros0 II Alocal.
+- unfold A.local in *. simpl in *. discriminate.
+- destruct a as [k v].
+  invc II. on >Forall2, invc. destruct y. break_and. simpl in *.
+  unfold A.local, B.local in *. simpl in *.
+
+  destruct (eq_nat_dec l k).
+  + inject_some.
+    eexists. break_if; try congruence. eauto.
+  + break_if; try congruence. eauto.
+Qed.
+
+Lemma eval_sim : forall af ae av bf be,
+    I_frame af bf ->
+    I_expr ae be ->
+    A.eval af ae av ->
+    exists bv,
+        B.eval bf be bv /\
+        I_value av bv.
+induction ae; intros0 IIframe IIexpr Aeval;
+inv IIframe; invc Aeval; invc IIexpr.
+
+- eexists. split. eapply B.EArg. auto.
+
+- eexists. split. eapply B.ESelf. auto.
+
+- fwd eapply local_sim; eauto. break_exists. break_and.
+  eexists. split. eapply B.EVar; eauto. auto.
+
+- fwd eapply IHae; eauto. break_exists. break_and.
+  on (I_value (V1.Constr _ _) _), invc.
+  fwd eapply Forall2_nth_error_ex; eauto. break_exists. break_and.
+  eexists. split. eapply B.EDerefConstr; eauto. auto.
+
+- fwd eapply IHae; eauto. break_exists. break_and.
+  on (I_value (V1.Close _ _) _), invc.
+  fwd eapply Forall2_nth_error_ex; eauto. break_exists. break_and.
+  eexists. split. eapply B.EDerefClose; eauto. auto.
+Qed.
+
+Lemma eval_sim_forall : forall af aes avs bf bes,
+    I_frame af bf ->
+    Forall2 I_expr aes bes ->
+    Forall2 (A.eval af) aes avs ->
+    exists bvs,
+        Forall2 (B.eval bf) bes bvs /\
+        Forall2 I_value avs bvs.
+first_induction aes; intros0 IIframe IIexpr Aeval;
+invc IIexpr; invc Aeval.
+- exists []. eauto.
+- fwd eapply eval_sim; eauto. break_exists. break_and.
+  fwd eapply IHaes; eauto. break_exists. break_and.
+  eexists. eauto.
+Qed.
+
+Lemma numbered_zlookup' : forall A base xs n (x : A),
+    (base <= n) ->
+    nth_error xs (n - base) = Some x ->
+    zlookup (numbered (Z.of_nat base) xs) (Z.of_nat n) = Some x.
+first_induction xs; intros0 Hle Hnth; simpl in *.
+- destruct (n - base); discriminate.
+- break_if.
+  + rewrite Nat2Z.inj_iff in *. subst base.
+    replace (n - n) with 0 in * by lia.
+    simpl in *. auto.
+  + rewrite <- Nat2Z.inj_succ.
+    eapply IHxs.
+      { rewrite Nat2Z.inj_iff in *. lia. }
+    destruct (n - base) eqn:?.
+      { exfalso. lia. }
+    simpl in *.
+    replace (n - S base) with n1 by lia. auto.
+Qed.
+
+Lemma numbered_zlookup : forall A xs n (x : A),
+    nth_error xs n = Some x ->
+    zlookup (numbered 0 xs) (Z.of_nat n) = Some x.
+intros.
+change 0%Z with (Z.of_nat 0).
+eapply numbered_zlookup'.
+- lia.
+- replace (n - 0) with n by lia. auto.
+Qed.
+
+Theorem I_sim : forall AE BE a a' b,
+    Forall2 I_func AE BE ->
+    I a b ->
+    A.sstep AE a a' ->
+    exists b',
+        B.sstep BE b b' /\
+        I a' b'.
+destruct a as [ae af ak | val ak | ae];
+intros0 Henv II Astep; [ | | solve [invc Astep] ];
+inv Astep; inv II;
+try on >I_stmt, invc;
+try on >I_frame, inv;
+simpl in *.
+
+- (* Seq *)
+  eexists. split. eapply B.SSeq; eauto.
+  i_ctor. i_ctor.
+
+- (* MkConstr *)
+  fwd eapply eval_sim_forall; eauto. break_exists. break_and.
+  eexists. split. eapply B.SConstrDone; eauto.
+  i_ctor. i_lem set_I_frame. i_ctor.
+
+- (* MkClose *)
+  fwd eapply eval_sim_forall; eauto. break_exists. break_and.
+  eexists. split. eapply B.SCloseDone; eauto.
+  i_ctor. i_lem set_I_frame. i_ctor.
+
+- (* MakeCall *)
+  fwd eapply Forall2_nth_error_ex with (xs := AE) as HH; eauto.
+    destruct HH as ([bbody bret] & ? & ?).
+  on >I_func, invc.
+
+  fwd eapply eval_sim with (ae := fe); eauto. break_exists. break_and.
+  fwd eapply eval_sim with (ae := ae0); eauto. break_exists. break_and.
+  on (I_value (V1.Close _ _) _), invc.
+
+  eexists. split. eapply B.SMakeCall; eauto.
+    { rewrite SuccNat2Pos.id_succ. simpl. eauto. }
+  i_ctor.
+  + i_ctor. i_ctor.
+  + i_ctor. i_ctor.
+
+- (* Switchinate *)
+  fwd eapply Forall2_nth_error_ex with (xs := cases) as HH; eauto.  destruct HH as (bcase & ? & ?).
+
+  subst aarg. on (I_value (V1.Constr _ _) _), invc.
+
+  eexists. split. eapply B.SSwitchinate; eauto using eq_refl.
+    { on (_ = Int.unsigned _), fun H => rewrite <- H. eauto using numbered_zlookup. }
+  i_ctor. i_ctor.
+
+- (* Assign *)
+  fwd eapply eval_sim; eauto. break_exists. break_and.
+  eexists. split. eapply B.SAssign; eauto.
+  i_ctor.
+
+
+- (* ContSeq *)
+  on >I_cont, inv.
+
+  eexists. split. eapply B.SContSeq; eauto.
+  i_ctor.
+
+- (* ContSwitch *)
+  on >I_cont, inv.
+
+  eexists. split. eapply B.SContSwitch; eauto.
+  i_ctor.
+
+- (* ContReturn *)
+  on >I_cont, inv.
+  fwd eapply eval_sim; eauto. break_exists. break_and.
+
+  eexists. split. eapply B.SContReturn; eauto.
+  i_ctor.
+
+- (* ContStop *)
+  on >I_cont, inv.
+  fwd eapply eval_sim; eauto. break_exists. break_and.
+
+  eexists. split. eapply B.SContStop; eauto.
+  i_ctor.
+
+- (* ContCall *)
+  on >I_cont, inv.
+
+  eexists. split. eapply B.SContCall; eauto.
+  i_ctor.
+Qed.
